theories/TLCbuffer.v
@@ -99,6 +99,23 @@ Qed.
 
 
 (*----------------------*)
+(* LibInt *)
+
+Definition max (n m:int) : int := 
+  If n > m then n else m.
+
+Lemma max_nonpos : forall n,
+  n <= 0 ->
+  max 0 n = 0.
+Proof using. introv M. unfold max. case_if; math. Qed.
+
+Lemma max_nonneg : forall n,
+  n >= 0 ->
+  max 0 n = n.
+Proof using. introv M. unfold max. case_if; math. Qed.
+
+
+(*----------------------*)
 (* LibLogic *)
 
 Lemma if_classicT_eq_if_isTrue : forall A (X Y:A) (P:Prop),
